WIP: step progress

theories/steps_progress.v
@@ -26,23 +26,113 @@ Proof.
   intros. by apply (not_elem_of_dom (D:=gset loc)), is_fresh_block.
 Qed.
 
-Definition borrow_write_match (bor: borrow) (stack: bstack) :=
+Definition borrow_write_match (bor: borrow) (stack: list stack_item) :=
   match bor with
-  | UniqB t => Uniq t ∈ stack.(borrows)
-  | AliasB _ => Raw ∈ stack.(borrows)
+  | UniqB t => Uniq t ∈ stack
+  | AliasB _ => Raw ∈ stack
   end.
 
-Lemma dealloc_head_step σ T l bor
+Lemma list_find_None_inv {A} (P : A → Prop) `{∀ x, Decision (P x)} l :
+  Forall (λ x, ¬ P x) l → list_find P l = None.
+Proof.
+  induction l as [|x l IHl]; [eauto|]. simpl. intros FA.
+  rewrite decide_False; [|apply (Forall_inv FA)]. rewrite IHl; [done|].
+  by eapply Forall_cons_1.
+Qed.
+
+Lemma dealloc_no_active_barrier_true stack β kind
+  (BAR: Forall (λ si, ¬ is_active_barrier β si) stack) :
+  dealloc_no_active_barrier kind stack β = true.
+Proof.
+  rewrite /dealloc_no_active_barrier. destruct kind; [done..|].
+  rewrite (_: find_top_active_call stack β = None); [done|].
+  by rewrite /find_top_active_call list_find_None_inv.
+Qed.
+
+Lemma access1'_dealloc_progress bor stack β
+  (BAR: Forall (λ si, ¬ is_active_barrier β si) stack)
+  (BOR: borrow_write_match bor stack) :
+  ∃ stack', access1' stack bor AccessDealloc β = Some stack'.
+Proof.
+  induction stack as [|si stack IH].
+  { exfalso. move : BOR. rewrite /borrow_write_match.
+    by destruct bor; apply not_elem_of_nil. }
+  destruct (Forall_cons_1 _ _ _ BAR) as [NA BAR'].
+  specialize (IH BAR').
+  destruct si as [t1| |c]; [destruct bor as [t2|ot]|destruct bor|].
+  - cbn -[dealloc_no_active_barrier]. case decide => ?.
+    + subst. rewrite dealloc_no_active_barrier_true; [by eexists|done].
+    + apply IH. by move : BOR => /elem_of_cons [[]|].
+  - apply IH. by move : BOR => /elem_of_cons [|].
+  - apply IH. by move : BOR => /elem_of_cons [|].
+  - cbn -[dealloc_no_active_barrier].
+    rewrite dealloc_no_active_barrier_true; [by eexists|done].
+  - rewrite /= /is_active bool_decide_false; [|done]. apply IH.
+    move : BOR; by destruct bor => /elem_of_cons [|].
+Qed.
+
+Lemma accessN_dealloc_progress α β l bor (n: nat) :
+  (∀ m : Z, 0 ≤ m ∧ m < n → l +ₗ m ∈ dom (gset loc) α) →
+  (∀ (m: nat) stack, (m < n)%nat →
+    α !! (l +ₗ m) = Some stack → borrow_write_match bor stack.(borrows) ∧ ∀ c,
+      FnBarrier c ∈ stack.(borrows) → β !! c = Some false) →
+  ∃ α', accessN α β l bor n AccessDealloc = Some α'.
+Proof.
+  revert α. induction n as [|n IHn]; intros α IN BOR; simpl; [by eexists|].
+  assert (is_Some (α !! (l +ₗ n))) as [stack Eq].
+  { apply (elem_of_dom (D:=gset loc)), IN. by lia. }
+  rewrite Eq /=.
+  destruct (BOR n stack) as [BM FB]; [lia|done|..].
+  assert (is_Some (access1' stack.(borrows) bor AccessDealloc β)) as [stk' Eq'].
+  { apply access1'_dealloc_progress; [|done].
+    apply Forall_forall. intros [t1| |c]; simpl; naive_solver. }
+  assert (is_Some (access1 β stack bor AccessDealloc)) as [stack' Eq2].
+  { rewrite /access1. case frozen_since as [tf|]; rewrite Eq'; by eexists. }
+  rewrite Eq2 /=. apply IHn.
+  - intros. apply elem_of_dom. rewrite lookup_delete_ne.
+    + apply (elem_of_dom (D:=gset loc)), IN. lia.
+    + move => /shift_loc_inj. lia.
+  - intros ???. rewrite lookup_delete_ne.
+    + apply BOR. lia.
+    + move => /shift_loc_inj. lia.
+Qed.
+
+Lemma dealloc_head_step (σ: state) T l bor
+  (WF: Wf σ)
   (BLK: ∀ m : Z, l +ₗ m ∈ dom (gset loc) σ.(cheap) ↔ 0 ≤ m ∧ m < tsize T)
   (BOR: ∀ (n: nat) stack, (n < tsize T)%nat →
-    σ.(cstk) !! (l +ₗ n) = Some stack → borrow_write_match bor stack ∧ ∀ c,
-      FnBarrier c ∈ stack.(borrows) → σ.(cbar) !! c = Some false) :
+    σ.(cstk) !! (l +ₗ n) = Some stack → borrow_write_match bor stack.(borrows) ∧
+    ∀ c, FnBarrier c ∈ stack.(borrows) → σ.(cbar) !! c = Some false) :
   ∃ σ',
   head_step (Free (Place l bor T)) σ [DeallocEvt l bor T] #☠ σ' [].
 Proof.
-  eexists. econstructor; econstructor.
-  - intros. by rewrite -(elem_of_dom (D:= gset loc) σ.(cheap)).
-  -
+  destruct (accessN_dealloc_progress σ.(cstk) σ.(cbar) l bor (tsize T))
+    as [α' Eq']; [|done|].
+  - intros. rewrite -(state_wf_dom _ WF). by apply BLK.
+  - eexists. econstructor; econstructor; [|done].
+    intros. by rewrite -(elem_of_dom (D:= gset loc) σ.(cheap)).
+Qed.
+
+Lemma copy_head_step σ l bor T :
+  ∃ σ' vl,
+  head_step (Copy (Place l bor T)) σ
+            [CopyEvt l bor T vl] (of_val (TValV vl)) σ' [].
+Proof.
+Abort.
+
+Lemma write_head_step σ l bor T el vl
+  (VALUES: to_val (TVal el) = Some (TValV vl)) :
+  ∃ σ',
+  head_step (Write (Place l bor T) (TVal el)) σ
+            [WriteEvt l bor T vl] #☠ σ' [].
+Proof.
+Abort.
+
+Lemma deref_head_step σ l bor T mut :
+  ∃ σ',
+  head_step (Deref (Lit (LitLoc l bor)) T mut) σ
+            [DerefEvt l bor T mut] (Place l bor T) σ' [].
+Proof.
 Abort.
 
 Lemma newcall_head_step σ :
@@ -55,6 +145,12 @@ Lemma endcall_head_step σ c (NZ: 0 ≤ c)
   ∃ σ',
   head_step (EndCall #c) σ [EndCallEvt (Z.to_nat c)] #☠ σ' [].
 Proof. eexists. econstructor; econstructor. lia. done. Qed.
+
+Lemma retag_head_step σ x xbor T kind :
+  ∃ σ',
+  head_step (Retag (Place x xbor T) kind) σ [RetagEvt x T kind] #☠ σ' [].
+Proof.
+Abort.
 
 Lemma syscall_head_step σ id :
   head_step (SysCall id) σ [SysCallEvt id] #☠ σ [].
